theories/prob_eff_lang/probblaze/typing/fundamental_subtyping.v
@@ -1,0 +1,580 @@
+From clutch.prob_eff_lang.probblaze.typing Require Import interp types.
+From clutch.prob_eff_lang.probblaze Require Import logic sem_types sem_sig sem_row mode sem_def sem_env.
+
+Section aux_lemma.
+  Context `{!probblazeRGS Σ}.
+ Lemma arr_extend_D ρ' D η μ δ ξ : 
+     erase_ctx η μ δ ξ D -∗ distinct' (iLblSig_to_iLblThy (interp._row η μ δ ρ' ξ)) -∗
+     logic.valid (iLblSig_to_iLblThy (interp._row η μ δ ρ' ξ)) -∗
+     erase_ctx η μ δ ξ (le.update_disj_ctx ρ' D).
+  Proof.
+    iIntros "#HD #Hd #Hv".
+    iDestruct (erase_ctx_row_to_disj_ctx η μ δ ξ ρ' with "[$Hv $Hd]")
+      as "#Hrow".
+    rewrite /erase_ctx /le.update_disj_ctx /le.merge_ctx.
+    iIntros "!#" (s ss js ρ0 Hlk Hc Ha).
+    apply lookup_union_with_Some in Hlk as [(Hlk1&Hlk2) | [(Hlk1&Hlk2) | Hb]].
+    (* [row_to_disj_ctx ρ'] only: discharge directly from [Hrow]. *)
+    1: by iApply ("Hrow" $! s ss js ρ0 with "[//] [//] [//]").
+    (* [D] only: discharge directly from [HD]. *)
+    1: by iApply ("HD" $! s ss js ρ0 with "[//] [//] [//]").
+    (* Both: the merged entry has [ss = ss1 ∪ ss2], [js = js1 ∪ js2].  Every
+       concrete name / row variable of [ρ0] lands in one of the two summands,
+       so freshness of [(δ !!! s)] against [ρ0] is reconstructed element-wise
+       from the per-side facts [Hm1] ([Hrow]) and [Hm2] ([HD]). *)
+    destruct Hb as ([ss1 js1] & [ss2 js2] & Hlk1 & Hlk2 & Heq).
+    simpl in Heq. injection Heq as <- <-.
+    iAssert (⌜∀ ρa, le.conc_sigs ρa ⊆ ss1 → le.abst_sigs ρa ⊆ js1 →
+      (δ !!! s).1 ∉ row_labels_l ρa ξ δ
+      ∧ (δ !!! s).2 ∉ row_labels_r ρa ξ δ⌝)%I as %Hm1.
+    { iIntros (ρa Hca Haa).
+      iDestruct ("Hrow" $! s ss1 js1 ρa with "[//] [//] [//]")
+        as "(_ & _ & %Hfl & %Hfr)".
+      rewrite (labels_l_interp_row ρa η μ δ ξ) in Hfl.
+      rewrite (labels_r_interp_row ρa η μ δ ξ) in Hfr.
+      iPureIntro; split; assumption. }
+    iAssert (⌜∀ ρa, le.conc_sigs ρa ⊆ ss2 → le.abst_sigs ρa ⊆ js2 →
+      (δ !!! s).1 ∉ row_labels_l ρa ξ δ
+      ∧ (δ !!! s).2 ∉ row_labels_r ρa ξ δ⌝)%I as %Hm2.
+    { iIntros (ρa Hca Haa).
+      iDestruct ("HD" $! s ss2 js2 ρa with "[//] [//] [//]")
+        as "(_ & _ & %Hfl & %Hfr)".
+      rewrite (labels_l_interp_row ρa η μ δ ξ) in Hfl.
+      rewrite (labels_r_interp_row ρa η μ δ ξ) in Hfr.
+      iPureIntro; split; assumption. }
+    (* Ownership does not depend on [ρ0]; read it off [D] at the empty row. *)
+    assert (Hc0 : le.conc_sigs RNil ⊆ ss2)
+      by (cbn [le.conc_sigs]; multiset_solver).
+    assert (Ha0 : le.abst_sigs RNil ⊆ js2)
+      by (cbn [le.abst_sigs]; set_solver).
+    iDestruct ("HD" $! s ss2 js2 RNil with "[//] [//] [//]")
+      as "(#Hown1 & #Hown2 & _)".
+    iSplit; [iApply "Hown1"|].
+    iSplit; [iApply "Hown2"|].
+    iSplit.
+    - iPureIntro.
+      rewrite (labels_l_interp_row ρ0 η μ δ ξ).
+      intros Hin. rewrite row_labels_l_split elem_of_app in Hin.
+      destruct Hin as [Hn | Hvr].
+      + rewrite /name_labels_l list_elem_of_fmap in Hn.
+        destruct Hn as (t & Heqt & Ht). apply gmultiset_elem_of_elements in Ht.
+        assert (Htu : t ∈ ss1 ∪ ss2)
+          by (eapply gmultiset_elem_of_subseteq; eauto).
+        apply gmultiset_elem_of_union in Htu as [Ht1 | Ht2].
+        * assert (Hp1 : le.conc_sigs (RCons (SSig t TBot TBot) RNil) ⊆ ss1)
+            by (cbn [le.conc_sigs le.eff_name_from_sig]; multiset_solver).
+          assert (Hp2 : le.abst_sigs (RCons (SSig t TBot TBot) RNil) ⊆ js1)
+            by (cbn [le.abst_sigs]; set_solver).
+          destruct (Hm1 _ Hp1 Hp2) as [Hnl _].
+          apply Hnl. cbn [row_labels_l le.eff_name_from_sig].
+          rewrite Heqt. apply list_elem_of_here.
+        * assert (Hp1 : le.conc_sigs (RCons (SSig t TBot TBot) RNil) ⊆ ss2)
+            by (cbn [le.conc_sigs le.eff_name_from_sig]; multiset_solver).
+          assert (Hp2 : le.abst_sigs (RCons (SSig t TBot TBot) RNil) ⊆ js2)
+            by (cbn [le.abst_sigs]; set_solver).
+          destruct (Hm2 _ Hp1 Hp2) as [Hnl _].
+          apply Hnl. cbn [row_labels_l le.eff_name_from_sig].
+          rewrite Heqt. apply list_elem_of_here.
+      + destruct (elem_of_var_labels_l_mono ρ0 ρ0 ξ _ (reflexivity _) Hvr)
+          as (i & Hi & Hl).
+        assert (Hiu : i ∈ js1 ∪ js2) by (eapply elem_of_weaken; eauto).
+        apply elem_of_union in Hiu as [Hi1 | Hi2].
+        * assert (Hp1 : le.conc_sigs (RVar i) ⊆ ss1)
+            by (cbn [le.conc_sigs]; multiset_solver).
+          assert (Hp2 : le.abst_sigs (RVar i) ⊆ js1)
+            by (cbn [le.abst_sigs]; set_solver).
+          destruct (Hm1 _ Hp1 Hp2) as [Hnl _].
+          apply Hnl. cbn [row_labels_l]. exact Hl.
+        * assert (Hp1 : le.conc_sigs (RVar i) ⊆ ss2)
+            by (cbn [le.conc_sigs]; multiset_solver).
+          assert (Hp2 : le.abst_sigs (RVar i) ⊆ js2)
+            by (cbn [le.abst_sigs]; set_solver).
+          destruct (Hm2 _ Hp1 Hp2) as [Hnl _].
+          apply Hnl. cbn [row_labels_l]. exact Hl.
+    - iPureIntro.
+      rewrite (labels_r_interp_row ρ0 η μ δ ξ).
+      intros Hin. rewrite row_labels_r_split elem_of_app in Hin.
+      destruct Hin as [Hn | Hvr].
+      + rewrite /name_labels_r list_elem_of_fmap in Hn.
+        destruct Hn as (t & Heqt & Ht). apply gmultiset_elem_of_elements in Ht.
+        assert (Htu : t ∈ ss1 ∪ ss2)
+          by (eapply gmultiset_elem_of_subseteq; eauto).
+        apply gmultiset_elem_of_union in Htu as [Ht1 | Ht2].
+        * assert (Hp1 : le.conc_sigs (RCons (SSig t TBot TBot) RNil) ⊆ ss1)
+            by (cbn [le.conc_sigs le.eff_name_from_sig]; multiset_solver).
+          assert (Hp2 : le.abst_sigs (RCons (SSig t TBot TBot) RNil) ⊆ js1)
+            by (cbn [le.abst_sigs]; set_solver).
+          destruct (Hm1 _ Hp1 Hp2) as [_ Hnr].
+          apply Hnr. cbn [row_labels_r le.eff_name_from_sig].
+          rewrite Heqt. apply list_elem_of_here.
+        * assert (Hp1 : le.conc_sigs (RCons (SSig t TBot TBot) RNil) ⊆ ss2)
+            by (cbn [le.conc_sigs le.eff_name_from_sig]; multiset_solver).
+          assert (Hp2 : le.abst_sigs (RCons (SSig t TBot TBot) RNil) ⊆ js2)
+            by (cbn [le.abst_sigs]; set_solver).
+          destruct (Hm2 _ Hp1 Hp2) as [_ Hnr].
+          apply Hnr. cbn [row_labels_r le.eff_name_from_sig].
+          rewrite Heqt. apply list_elem_of_here.
+      + destruct (elem_of_var_labels_r_mono ρ0 ρ0 ξ _ (reflexivity _) Hvr)
+          as (i & Hi & Hl).
+        assert (Hiu : i ∈ js1 ∪ js2) by (eapply elem_of_weaken; eauto).
+        apply elem_of_union in Hiu as [Hi1 | Hi2].
+        * assert (Hp1 : le.conc_sigs (RVar i) ⊆ ss1)
+            by (cbn [le.conc_sigs]; multiset_solver).
+          assert (Hp2 : le.abst_sigs (RVar i) ⊆ js1)
+            by (cbn [le.abst_sigs]; set_solver).
+          destruct (Hm1 _ Hp1 Hp2) as [_ Hnr].
+          apply Hnr. cbn [row_labels_r]. exact Hl.
+        * assert (Hp1 : le.conc_sigs (RVar i) ⊆ ss2)
+            by (cbn [le.conc_sigs]; multiset_solver).
+          assert (Hp2 : le.abst_sigs (RVar i) ⊆ js2)
+            by (cbn [le.abst_sigs]; set_solver).
+          destruct (Hm2 _ Hp1 Hp2) as [_ Hnr].
+          apply Hnr. cbn [row_labels_r]. exact Hl.
+  Qed.
+
+End aux_lemma.
+
+Section compatiblity.
+  Context `{!probblazeRGS Σ}.
+  
+  Lemma sig_le_eff D α α' β β' s : 
+   sem_ty_le D α α' -∗ sem_ty_le D β' β -∗ sem_sig_le D (SSig s α β) (SSig s α' β').
+  Proof. 
+    iIntros "#Hα #Hβ !# %%%% #HD".
+    iApply sig_le_eff; iIntros (αs) "!#"; [iApply "Hα"|iApply "Hβ"]; 
+      by iApply erase_ctx_extend_ty.
+  Qed. 
+  
+  Lemma row_le_RNil D b :
+    ⊢ sem_row_le D b RNil RNil.
+  Proof. 
+    iIntros (????) "!# #He". 
+    iSplit; last iApply row_le_refl; by destruct b.
+  Qed. 
+
+  Lemma row_le_RVar D b i :
+    ⊢ sem_row_le D b (RVar i) (RVar i).
+  Proof. 
+    iIntros (????) "!# #He". 
+    iSplit; last iApply row_le_refl; by destruct b.
+  Qed. 
+
+  Lemma row_le_RExtend D b σ ρ : 
+    ⊢ sem_row_le D b ρ (RCons σ ρ).
+  Proof. 
+    iIntros (????) "!# #He". 
+    iSplit; last iApply row_le_cons_extend; destruct b; try done; iPureIntro; split;
+    solve_submseteq.
+  Qed. 
+
+  Lemma row_le_RSwap D b σ σ' ρ :
+    ⊢ sem_row_le D b (RCons σ (RCons σ' ρ)) (RCons σ' (RCons σ ρ)).
+  Proof. 
+    iIntros (????) "!# #He". 
+    iSplit.
+    - iPureIntro; destruct b; try done; split; solve_submseteq.
+    - iApply row_le_swap_second.
+  Qed. 
+
+  Lemma row_le_RCons D b σ σ' ρ ρ' :
+    sem_sig_le D σ σ' -∗
+    sem_row_le D false ρ ρ' -∗
+    sem_row_le D b (RCons σ ρ) (RCons σ' ρ').
+  Proof. 
+    iIntros "#Hsig #Hrow %%%% !# #HD".
+    iDestruct ("Hsig" with "HD") as "(%Hsig&_)".
+    rewrite !sig_labels_eff_name in Hsig. 
+    iDestruct ("Hrow" with "HD") as "(%Hlabel&Hrow')".
+    destruct Hlabel as [Hll Hlr].
+    iSplit.
+    - iPureIntro; destruct b; try done; split.
+      + rewrite //= Hsig; by apply submseteq_skip.
+      + rewrite //= Hsig; by apply submseteq_skip.
+    - iApply row_le_cons_comp.
+      + by rewrite !labels_l_interp_row. 
+      + by rewrite !labels_r_interp_row. 
+      + by iApply "Hsig".
+      + by iApply "Hrow'".
+  Qed. 
+    
+  Lemma row_le_RUnion D b ρ1 ρ2 ρ1' ρ2' :
+    sem_row_le D false ρ1 ρ1' -∗
+      sem_row_le D false ρ2 ρ2' -∗
+      sem_row_le D b (ρ1 ∪ᵣ ρ2)%ty (ρ1' ∪ᵣ ρ2')%ty.
+  Proof. 
+    iIntros "#Hrow1 #Hrow2 %%%% !# #HD".
+    iDestruct ("Hrow1" with "HD") as "(%Hl1&Hrow1')".
+    destruct Hl1 as [Hll1 Hlr1].
+    iDestruct ("Hrow2" with "HD") as "(%Hl2&Hrow2')".
+    destruct Hl2 as [Hll2 Hlr2].
+    iSplit.
+    - iPureIntro; destruct b; try done.
+      split; simpl; by apply submseteq_app.
+    - iApply row_le_union'.
+      + by rewrite !labels_l_interp_row. 
+      + by rewrite !labels_l_interp_row. 
+      + by rewrite !labels_r_interp_row. 
+      + by rewrite !labels_r_interp_row. 
+      + by iApply "Hrow1'".
+      + by iApply "Hrow2'".
+  Qed. 
+
+  Lemma row_le_RErase D s ss js ρ :
+    ⌜D !! s = Some (ss, js)⌝ -∗
+    ⌜le.conc_sigs ρ ⊆ ss⌝ -∗
+    ⌜le.abst_sigs ρ ⊆ js⌝ -∗
+    sem_row_le D true (RCons (SAbs s) ρ) ρ.
+  Proof. 
+    iIntros (Hin Hcnc Habs ????) "!# #HD".
+    iSplit; first done.
+    iDestruct ("HD" $! s ss js ρ with "[//] [//] [//]")
+      as "(Hl1 & Hl2 & %Hnl & %Hnr)".
+    by iApply row_le_erase.
+  Qed. 
+
+  Lemma row_le_RTrans D b ρ1 ρ2 ρ3 :
+    sem_row_le D b ρ1 ρ2 -∗
+    sem_row_le D b ρ2 ρ3 -∗
+    sem_row_le D b ρ1 ρ3.
+  Proof. 
+    iIntros "#Hrow1 #Hrow2 %%%% !# #HD".
+    iDestruct ("Hrow1" with "HD") as "(%Hl1&Hrow1')".
+    iDestruct ("Hrow2" with "HD") as "(%Hl2&Hrow2')".
+    iSplit.
+    - iPureIntro; destruct b; first done.
+      destruct Hl1 as [Hll1 Hlr1].
+      destruct Hl2 as [Hll2 Hlr2]. 
+      split; by eapply submseteq_trans.
+    - by iApply row_le_trans.
+  Qed. 
+
+  Lemma row_le_RFlipNil D b m :
+    ⊢ sem_row_le D b (¡[ m] RNil) RNil.
+  Proof. 
+    iIntros (????) "!# #HD".
+    iSplit; first (by destruct b).
+    iApply row_le_mfbang_elim_nil.
+  Qed. 
+
+  Lemma row_le_RFlipCons D b m σ ρ :
+    ⊢ sem_row_le D b (¡[ m] (RCons σ ρ)) (RCons (SFlip m σ) (¡[ m] ρ)).
+  Proof. 
+    iIntros (????) "!# #HD".
+    iSplit; first (by destruct b).
+    iApply row_le_mfbang_dist_cons.
+  Qed. 
+
+  Lemma row_le_RFlipUnion D b m ρ1 ρ2 :
+    ⊢ sem_row_le D b (¡[ m] (ρ1 ∪ᵣ ρ2)%ty) (¡[ m] ρ1 ∪ᵣ ¡[ m] ρ2)%ty.
+  Proof. 
+    iIntros (????) "!# #HD".
+    iSplit; first (by destruct b).
+    iApply row_le_flip_union.
+  Qed. 
+  
+  Lemma row_le_RFlipElim D b ρ :
+    ⊢ sem_row_le D b (¡[ types.MS] ρ) ρ.
+  Proof. 
+    iIntros (????) "!# #HD".
+    iSplit; first (by destruct b).
+    iApply row_le_mfbang_elim_ms.
+  Qed. 
+
+  Lemma row_le_RFlipIntro D b ρ m :
+    ⊢ sem_row_le D b ρ (¡[ m] ρ).
+  Proof. 
+    iIntros (????) "!# #HD".
+    iSplit; first (by destruct b).
+    iApply row_le_mfbang_intro.
+  Qed. 
+
+  Lemma row_le_RFlipIdemp1 D b ρ m :
+    ⊢ sem_row_le D b (¡[ m] (¡[ m] ρ)) (¡[ m] ρ).
+  Proof. 
+    iIntros (????) "!# #HD".
+    iSplit; first (by destruct b).
+    iApply row_le_mfbang_idemp.
+  Qed. 
+
+  Lemma row_le_RFlipIdemp2 D b ρ m :
+    ⊢ sem_row_le D b (¡[ m] ρ) (¡[ m] (¡[ m] ρ)).
+  Proof. 
+    iIntros (????) "!# #HD".
+    iSplit; first (by destruct b).
+    iApply row_le_mfbang_intro.
+  Qed. 
+
+  Lemma row_le_RFlipComp D b ρ ρ' m m' :
+    sem_mode_le m m' -∗
+    sem_row_le D b ρ' ρ -∗
+    sem_row_le D b (¡[ m'] ρ') (¡[ m] ρ).
+  Proof. 
+    iIntros "#Hmode #Hrow %%%% !# #HD".
+    iDestruct ("Hrow" with "HD") as "(%Hl&Hrow')".
+    iSplit.
+    - iPureIntro; destruct b; first done.
+      destruct Hl as [Hll Hlr].
+      split; by eapply submseteq_trans.
+    - by iApply row_le_mfbang_comp.
+  Qed. 
+
+  Lemma ty_le_TArrow D b α α' β β' ρ ρ' :
+    let D' := le.update_disj_ctx ρ' D in
+    sem_ty_le D' α' α -∗
+    sem_ty_le D' β β' -∗
+    sem_row_le D' b ρ ρ' -∗
+    sem_ty_le D (α -{ ρ }-∘ β) (α' -{ ρ' }-∘ β').
+  Proof. 
+    iIntros (?) "#Hty1 #Hty2 #Hrow %%%% !# #HD".
+    iIntros (??) "!# Hτ1 % % Hα". iApply brel_learn. 
+    iIntros "#Hd #Hv".
+    iRevert (w1 w2) "Hα".
+    iRevert (v1 v2) "Hτ1". 
+    iApply bi.intuitionistically_elim.
+    iDestruct (arr_extend_D with "[$HD]") as "#HD'".
+    iSpecialize ("HD'" with "Hd Hv"). 
+    iApply ty_le_arr.
+    - iDestruct ("Hrow" with "HD'") as "(_&$)".
+    - by iApply "Hty1". 
+    - by iApply "Hty2".
+  Qed. 
+
+  Lemma ty_le_TForall D α β :
+    sem_ty_le D α β -∗
+    sem_ty_le D (∀T: α) (∀T: β).
+  Proof. 
+    iIntros "#Hty %%%% !# #HD"; iApply ty_le_type_forall; iIntros (α'); iApply "Hty"; by iApply erase_ctx_extend_ty.
+  Qed. 
+
+  Lemma ty_le_MForall D α β :
+    sem_ty_le D α β -∗
+    sem_ty_le D (∀M: α) (∀M: β).
+  Proof. 
+    iIntros "#Hty %%%% !# #HD"; iApply ty_le_mode_forall; iIntros (m); iApply "Hty"; by iApply erase_ctx_extend_mode.
+  Qed. 
+
+  Lemma ty_le_TBangNat D m :
+     ⊢ sem_ty_le D ℕ (![ m] ℕ).
+  Proof. 
+    iIntros (????) "!# #HD".
+    iIntros "!#" (v1 v2) "#Hnat". rewrite /sem_ty_mbang.
+    iApply bi.intuitionistically_intuitionistically_if. by iModIntro.
+  Qed. 
+
+  Lemma ty_le_TNat_TInt D :
+    ⊢ sem_ty_le D ℕ ℤ.
+  Proof. 
+    iIntros (????) "!# #HD".
+    iIntros "!#" (v1 v2) "Hnat". iDestruct "Hnat" as (n) "[-> ->]".
+    by iExists (Z.of_nat n). 
+  Qed. 
+
+End compatiblity.
+
+Section fundamental_subtyping.
+  Context `{!probblazeRGS Σ}. 
+
+  Theorem fundamental_mode (m m' : vmode) :
+    (⊢ₗ m ≤M m') → ⊢ @sem_mode_le Σ m m'.
+  Proof.
+    intros Hm. induction Hm; iIntros "!# %". 
+    - iApply mode_le_OS.
+    - iApply mode_le_MS.
+    - iApply mode_le_trans.
+      + iApply IHHm1.
+      + iApply IHHm2.
+    - iApply mode_le_refl.
+  Qed.
+
+
+  Theorem fundamental_sig D σ σ' :
+    D ⊢ₗ σ ≤S σ' → ⊢ sem_sig_le D σ σ'
+    with fundamental_row D ρ ρ' b :
+      D ⊢ₗ ρ ≤R ρ' @ b → ⊢ sem_row_le D b ρ ρ'
+      with fundamental_type D α β :
+        D ⊢ₗ α ≤T β → ⊢ sem_ty_le D α β.
+  Proof. 
+    - induction 1; iIntros (????) "!# He".
+      + iApply sig_le_eff; last done; by iApply fundamental_type. 
+      + iApply sig_le_mfbang_intro.
+      + iApply sig_le_mfbang_elim_ms.
+      + iApply sig_le_mfbang_idemp.
+      + iApply sig_le_mfbang_intro.
+      + iApply sig_le_mfbang_comp. 
+        * by iApply fundamental_mode. 
+        * by iApply fundamental_sig.
+    - induction 1. 
+      + iApply row_le_RNil. 
+      + iApply row_le_RVar.
+      + iApply row_le_RExtend.
+      + iApply row_le_RSwap.
+      + iApply row_le_RCons.
+        * by iApply fundamental_sig.
+        * by iApply fundamental_row.
+      + iApply row_le_RUnion; by iApply fundamental_row.
+      + by iApply row_le_RErase. 
+      + iApply row_le_RTrans; by iApply fundamental_row.
+      + iApply row_le_RFlipNil.
+      + iApply row_le_RFlipCons.
+      + iApply row_le_RFlipUnion.
+      + iApply row_le_RFlipElim.
+      + iApply row_le_RFlipIntro.
+      + iApply row_le_RFlipIdemp1.
+      + iApply row_le_RFlipIdemp2.
+      + iApply row_le_RFlipComp.
+        * by iApply fundamental_mode.
+        * by iApply fundamental_row.
+    - induction 1.  
+      + iIntros (????) "!# #HD"; iApply ty_le_refl.
+      + iIntros (????) "!# #HD"; iApply ty_le_trans; by iApply fundamental_type.
+      + iIntros (????) "!# #HD"; iApply ty_le_bot.
+      + by iIntros (????) "!# #HD !# % % _".
+      + by iApply ty_le_TArrow; last by iApply fundamental_row. 
+      + iIntros (????) "!# #HD"; iApply ty_le_ref; by iApply fundamental_type.
+      + by iApply ty_le_TForall.
+      + by iApply ty_le_MForall.
+      + iIntros (????) "!# #HD"; iApply ty_le_prod; by iApply fundamental_type.
+      + iIntros (????) "!# #HD"; iApply ty_le_sum; by iApply fundamental_type.
+      + iIntros (????) "!# #HD"; iApply ty_le_mbang_intro_bool.
+      + iIntros (????) "!# #HD"; iApply ty_le_mbang_intro_unit.
+      + iIntros (????) "!# #HD"; iApply ty_le_mbang_intro_int.
+      + iApply ty_le_TBangNat.
+      + iIntros (????) "!# #HD"; iApply ty_le_mbang_intro_top.
+      + iIntros (????) "!# #HD"; iApply ty_le_mbang_intro_os.
+      + iIntros (????) "!# #HD"; iApply ty_le_mbang_idemp.
+      + iIntros (????) "!# #HD"; iApply ty_le_mbang_elim.
+      + iIntros (????) "!# #HD"; iApply ty_le_mbang_elim.
+      + iIntros (????) "!# #HD"; iApply ty_le_mbang_comp.
+        * by iApply fundamental_mode.
+        * by iApply fundamental_type.
+      + iIntros (????) "!# #HD"; iApply ty_le_type_forall_mbang.
+      + iIntros (????) "!# #HD"; iApply ty_le_mbang_type_forall.
+      + iIntros (????) "!# #HD"; iApply ty_le_row_forall_mbang.
+      + iIntros (????) "!# #HD"; iApply ty_le_mbang_row_forall.
+      + iApply ty_le_TNat_TInt.
+  Qed. 
+  
+  Lemma multi_ty_sound (τ : type) :
+    le.MultiT τ → ∀ η μ δ ξ, MultiT (interp._ty η μ δ τ ξ).
+  Proof.
+    intros H ????. unfold le.MultiT in H. eapply fundamental_type in H.
+    constructor.
+    iApply H. iApply erase_ctx_empty.
+  Qed.
+
+  (* Soundness of [le.MultiC]: a syntactically multi context interprets to
+     a semantic [MultiE].  Forall-lift of [multi_ty_sound]. *)
+  Lemma multi_env_sound (Γ : ctx) :
+    le.MultiC Γ → ∀ η μ δ ξ, MultiE (interp._env η μ δ ξ Γ).
+  Proof.
+    intros Hm η μ δ ξ. induction Γ as [|[x τ] Γ' IH]; simpl.
+    - apply multi_env_nil.
+    - apply Forall_cons in Hm as [Hτ HΓ'].
+      apply multi_env_cons; first by apply IH.
+      by apply multi_ty_sound.
+  Qed.
+
+  (* Soundness of [le._mode_type]: note [m m⪯T τ] forces [m ∈ {OS, MS}]. *)
+  Lemma mode_type_sound (m : vmode) (τ : type) :
+    m m⪯T τ → ∀ η μ δ ξ, (interp._mode μ m) ₘ⪯ₜ (interp._ty η μ δ τ ξ).
+  Proof.
+    intros Hm η μ δ ξ. inv Hm; simpl.
+    - apply mode_type_sub_os.
+    - apply mode_type_sub_multi_ty. by apply multi_ty_sound.
+  Qed.
+
+  (* Soundness of [le._mode_ctx]: a syntactic mode-context judgement
+     interprets to a semantic mode-env-subtyping. *)
+  Lemma mode_env_sound (m : vmode) (Γ : ctx) :
+    m m⪯C Γ → ∀ η μ δ ξ, (interp._mode μ m) ₘ⪯ₑ (interp._env η μ δ ξ Γ).
+  Proof.
+    intros Hm η μ δ ξ. induction Hm as [m'|m' x τ Γ' Hτ HΓ' IH]; simpl.
+    - apply mode_env_sub_nil.
+    - destruct x as [|s]; simpl.
+      + apply IH.
+      + apply mode_env_sub_cons; first apply IH.
+        by apply mode_type_sound.
+  Qed.
+
+  Lemma once_row_sound (ρ : row) :
+    le.OnceR ρ → ∀ η μ δ ξ, OnceR (interp._row η μ δ ρ ξ).
+  Proof.
+    intros [b0 Hle] η0 μ0 ξ0. constructor.
+    iPoseProof (fundamental_row _ _ _ _ Hle) as "H".
+    iPoseProof erase_ctx_empty as "Hctx".
+    iDestruct ("H" with "Hctx") as "(_&$)".
+  Qed.
+
+  (* Soundness of [le._row_type]: turns [ρ R⪯T τ] into the semantic         *)
+  (* [RowTypeSub] typeclass.  The [Multi_le] case is fully proved (via      *)
+  (* [multi_ty_sound] + the existing [row_type_sub_multi_ty] instance); the *)
+  (* [Once_le] case is sound modulo [once_row_sound] above. *)
+  Lemma row_type_sub_sound (ρ : row) (τ : type) :
+    ρ R⪯T τ → ∀ η μ δ ξ,
+        RowTypeSub (interp._row η μ δ ρ ξ) (interp._ty η μ δ τ ξ).
+  Proof.
+    intros Hsub η0 μ0 δ0 ξ0. destruct Hsub as [ρ' τ' Honce | ρ' τ' Hmulti].
+    - apply row_type_sub_once.
+      by apply (once_row_sound _ Honce).
+    - pose proof (multi_ty_sound _ Hmulti η0 μ0 δ0 ξ0) as Hm.
+      by apply row_type_sub_multi_ty.
+  Qed.
+
+  (* Soundness of [le._row_ctx]: turns [ρ R⪯C Γ] into the semantic          *)
+  (* [RowEnvSub] typeclass.  Mirrors [mode_env_sound]: induction on the     *)
+  (* derivation, [Nil] via [row_env_sub_nil], [Cons] via [row_env_sub_cons] *)
+  (* fed by [row_type_sub_sound].  The [BAnon] binder leaves [Γ] unchanged. *)
+  Lemma row_env_sub_sound (ρ : row) (Γ : ctx) :
+    ρ R⪯C Γ → ∀ η μ δ ξ,
+        RowEnvSub (interp._row η μ δ ρ ξ) (interp._env η μ δ ξ Γ).
+  Proof.
+    intros Hsub η0 μ0 δ0 ξ0.
+    induction Hsub as [ρ'|ρ' x τ Γ' Hτ HΓ' IH]; simpl.
+    - apply row_env_sub_nil.
+    - destruct x as [|s]; simpl.
+      + apply IH.
+      + apply row_env_sub_cons; first apply IH.
+        by apply (row_type_sub_sound _ _ Hτ).
+  Qed.
+
+  (* Soundness of context subtyping [le._ctx].  The syntactic [D ⊢ₗ Γ ≤C Γ']
+     interprets to an [env_le] between the pointwise-interpreted contexts.
+     [le._ctx] recurses on [Γ'], so we induct on [Γ']: the [[]] case is the
+     unconditional [env_le_nil]; the cons case uses [env_le_bring_forth] to
+     surface the matched entry [(x,t')] out of [Γ = pre ++ (x,t') :: post],
+     [env_le_cons] with [ty_le_sound] on the head and the IH on the tail
+     (both under the [erase_ctx] bundle), combined by [env_le_trans]. *)
+  Lemma ctx_le_sound (D : le.disj_ctx) (Γ Γ' : ctx) :
+    D ⊢ₗ Γ ≤C Γ' → ⊢ sem_env_le D Γ Γ'.
+  Proof.
+    revert Γ. induction Γ' as [|[x t] Γ'_tail IH];
+      iIntros (Γ Hle) "!# %%%% #HD".
+    - iApply env_le_nil.
+    - simpl in Hle.
+      destruct Hle as (t' & pre & post & -> & Ht & Htail).
+      (* [(x,t')] sits at position [length pre] in the interpreted [Γ]. *)
+      assert (Hnth : nth_error ((λ '(s, τ), (s, interp._ty η μ δ τ ξ))
+                                  <$> (pre ++ (x, t') :: post))
+                       (length pre) = Some (x, interp._ty η μ δ t' ξ)).
+      { rewrite fmap_app /=. rewrite (nth_error_app2 _ _ (n := length pre)).
+        { rewrite length_fmap Nat.sub_diag //. }
+        rewrite length_fmap //. }
+      (* Deleting it leaves the interpretation of [pre ++ post]. *)
+      assert (Hdel : list_delete (length pre)
+                       ((λ '(s, τ), (s, interp._ty η μ δ τ ξ))
+                          <$> (pre ++ (x, t') :: post))
+                     = (λ '(s, τ), (s, interp._ty η μ δ τ ξ)) <$> (pre ++ post)).
+      { rewrite !fmap_app /=.
+        rewrite -(length_fmap (λ '(s, τ), (s, interp._ty η μ δ τ ξ)) pre).
+        apply delete_middle. }
+      simpl.
+      iApply (env_le_trans _ ((x, interp._ty η μ δ t' ξ)
+                                :: ((λ '(s, τ), (s, interp._ty η μ δ τ ξ)) <$> (pre ++ post)))).
+      + rewrite -Hdel.
+        iApply (env_le_bring_forth _ (length pre) x (interp._ty η μ δ t' ξ) Hnth).
+      + iApply env_le_cons.
+        * iApply (IH _ Htail with "HD").
+        * by iApply fundamental_type.  
+  Qed.
+
+End fundamental_subtyping.
